---
title: "Mathematical Analysis IB"
author: "Matt Alejo"
output:
  html_document:
    toc: yes
    toc_depth: '3'
    df_print: paged
  output:
    html_document: null
    toc: yes
    toc_depth: 2
---

# Review on differentiation

## Differentiability

Let $f$ be a function on some open interval $I$ containing $x$. The derivative of $f$ at $x$, denoted by $f'(x)$, is

$$ f'(x) = \lim_{h\to 0}\frac{f(x+h)-f(x)}{h} $$

## Differentiation rules

1. $\frac{d}{dx}(cf(x))= cf'(x)$

2. $\frac{d}{dx}(f(x) \pm g(x)) = f'(x) \pm g'(x)$

3. $\frac{d}{dx}(f(x)g(x)) = f(x)g'(x) + g(x)f'(x)$

4. $\frac{d}{dx}\frac{f(x)}{g(x)} = \frac{g(x)f'(x)-f(x)g'(x)}{(g(x))^2}$

5. $\frac{d}{dx}(f(g(x))) = f'(g(x))g'(x)$


## Differentiation formulas I

1. $\frac{d}{dx}(c)=0, c \in \mathbb{R}$

2. $\frac{d}{dx}(x^r)=rx^{r-1}, r \in \mathbb{R}$

3. $\frac{d}{dx}(sinx)=cos x$ 

4. $\frac{d}{dx}(cosx)=-sin x$

5. $\frac{d}{dx}(tanx)=sec^2x$

6. $\frac{d}{dx}(cotx)=-csc^x$

7. $\frac{d}{dx}(secx) = secxtanx$

8. $\frac{d}{dx}(cscx)=-cscxcotx$

## Differentiation formulas II

1. $\frac{d}{dx}(e^x) = e^x$

2. $\frac{d}{dx}(ln|x|) = \frac{1}{x}$

3. $\frac{d}{dx}(sin^{-1}x) = \frac{1}{\sqrt{1-x^2}}$

4. $\frac{d}{dx}(tan^{-1}x) = \frac{1}{1+x^2}$

5. $\frac{d}{dx}(sec^{-1}x) = \frac{1}{x \sqrt{x^2-1}}$

## Mean value theorem

Let $f$ be a function that is continuous on $[a,b]$ and is differentiable on $(a,b)$. Then there is a number $c\in(a,b)$ such that

$$ f'(c)=\frac{f(b)-f(a)}{b-a} $$

## Consequences of MVT

### Zero Derivative

If $f'(x)=0 \;\forall x$ in interval $I$, then $f(x)=c \;\forall x\in I$ for some constant $C$.

### Equal derivatives

If $f'(x)-g'(x)=0 \;\forall x$ in an interval $I$, then $f(x)=g(x)+C$ for some constant $C$.

#### Example

Let $f(x)=cos^{-1}x$ and $g(x)=-sin^{-1}x$

This implies that $x \in [-1,1]$ and $f(x),g(x) \in [-\frac{\pi}{2},\frac{\pi}{2}]$

$$ f'(x)=-\frac{1}{\sqrt{x^2+1}}$$

$$ g'(x)=-\frac{1}{\sqrt{x^2+1}} $$
Since $f'(x)-g'(x)=0$ for $x \in [-1,1]$, then $f(x)-g(x)=C$ for some constant $C$ by a corollary.

$$ cos^{-1}x - (-sin^{-1}x)=C $$
$$ cos^{-1}x +sin^{-1}x=C $$
Substituting $x \in [-1,1]$, in this case, let's use $x=0$,

$$ cos^{-1}(0) +sin^{-1}(0)=C $$
$$ 0 + \frac{\pi}{2} = C $$

$$ C = \frac{\pi}{2} $$ 

$$ \therefore \forall x \in[-1,1],f(x)-g(x)= \frac{\pi}{2}$$

## Differentials

$$ f'(x)=\frac{dy}{dx} $$
$$ dy = f'(x)dx $$


# Module 1: Indefinite and definite integrals

## Antiderivatives



## Substitution rule

## The area problem

## The definite Integrals

## The Fundamental Theorem of Calculus

## Proof of Fundamental Theorem of Calculus




# Module 2: Application I

## Areas between curves

## Volumes and volumes of revolution using disks and washers

## Volumes of solids of revolution using cylindrical shells

# Module 3: Techniques of integration

## Integration by parts

## Trigonometric integrals

## Trigonometric Substitution

## Partial fractions




# Applications II

## Arc length

## Variable-separable differential equations and models for population growthe editor.
